wonderful

automata.v
@@ -2,198 +2,287 @@ Require Import ssreflect ssrbool eqtype fintype finfun seq fingraph ssrfun.
 
 Set Implicit Arguments.
 
+(* Finite automata. *)
 Section FA.
-Variable S: finType.
-Definition word := seq S.
+(* input alphabet. *)
+Variable char: finType.
+(* Type of input sequences *)
+Definition word := seq char.
 
-
+(* Deterministic finite automata.
+   This is the only actual type of automata.
+   NFAs will be translated on the fly (they
+   never exist as instances of some type). *)
 Section DFA.
-Variable Q: finType.
-Definition dfa_rel (d: Q -> S -> Q) := (fun x y => existsb a, d x a == y).
-Inductive dfa (s0: Q) (f: pred Q) : rel Q  -> Type :=
-| dfaI  (d: Q -> S -> Q) : dfa s0 f 
-(dfa_rel d).
 
+(* The (finite) type of states *)
+Variable state: finType.
+
+(* The inductive type of deterministic finite automata *)
+Inductive dfa (s0: state) (fin: pred state) (step: state -> char -> state) : Type :=
+    | dfaI : dfa s0 fin step.
+
+
+(* Acceptance on DFAs *)
 Section Acceptance.
-Variable s0: Q.
-Variable f: pred Q.
-Definition AutR {R} (_: dfa s0 f R) := R.
 
-Variable R': rel Q.
-Variable A: dfa s0 f R'.
+(* Assume some automaton *)
+Variable s0_: state.
+Variable fin_: pred state.
+Variable step_: state -> char -> state.
+Variable A: dfa s0_ fin_ step_.
 
-Let R := AutR A.
-Definition d: Q -> S -> Q. elim: A => //. Defined.
+(* This is a giant, steaming pile of hack.
+   (It forces all the following functions to
+   take an automaton as argument.) *)
+Definition A_s0 := [fun A: dfa s0_ fin_ step_ => s0_ ].
+Definition A_fin := [ fun A: dfa s0_ fin_ step_ => fin_ ].
+Definition A_step := [ fun A: dfa s0_ fin_ step_ => step_ ].
+Let s0 := A_s0 A.
+Let fin := A_fin A.
+Let step := A_step A.
 
+(* We define a run of w on the automaton A
+   to be the list of states x_1 .. x_|w|
+   traversed when following the edges labeled
+   w_1 .. w_|w| starting in x. *)
+Fixpoint run' (x: state) (w: word) : seq state :=
+match w with
+  | [::] => [::]
+  | a::w => (step x a) ::run' (step x a) w
+end.
 
-Fixpoint accept_state' (q: Q) (w: word): Q. 
-Proof. move: q. elim: w => [ | a w IHw ]. 
-  by [].
-move => q. move: (d q a) w. exact: accept_state'. 
-Defined.
-Hint Resolve accept_state'.
+(* A simplifying function for a "complete" run
+   (i.e. starting at s0). *)
+Definition run := [fun w => run' s0 w].
+
+(* Acceptance of w in x is defined as
+   finality of the last state of a run of w on A
+   starting in x. *)
+Definition accept' := [ fun x w => fin (last x (run' x w) ) ].
+
+(* Acceptance of w on A starting in s0. *)
+Definition accept := [fun w => accept' s0 w].
+
+(* A lemma that helps us avoid cumbersome unfolding of accept' *)
+Lemma accept'S x a w : accept' x (a::w) = accept' (step x a) w.
+Proof. elim: w x a => [|b w IHw] x a //=. Qed.
+(* Same for accept. *)
+Lemma acceptS a w : accept (a::w) = accept' (step s0 a) w.
+Proof. elim: w a => [|b w IHw] a //=. Qed.
   
-(* dfa A accepts word w starting in state q *)
-Fixpoint accept' (q: Q) (w: word): bool.
-(* := f (accept_state' q w). *)
-Proof. move: q. elim: w => [ | a w IHw ]. 
-  exact: (f).
-move => q. exact: (accept' (d q a) w).
-Defined.
-
-Lemma accept_correct q w : accept' q w = f (accept_state' q w).
-Proof. elim: w q => [ | a w IHw ] q //=. Qed.
-
-Definition accept_state (w: word) := accept_state' s0 w.
-  
-Definition accept (w: word) := 
-accept' s0 w.
-
-Lemma d_connect q a: connect R q (d q a).
-Proof. unfold R. rewrite/d. elim: A => /= d0. rewrite/AutR. 
-apply/connect1. apply/existsP. by exists a.
+(* The size of a run is the size of the input word. *)
+Lemma run_size x w : size (run' x w) = size w.
+Proof. elim: w x => [|a w IHw] x //=.
+  by rewrite IHw.
 Qed.
 
-Definition sink q := forallb q', connect R q q' ==> ~~ f q'.
+(* Predicate to distinguish between accepting
+   and non-accepting runs. *)
+Definition run_accepts x xs := fin (last x xs).
 
-Lemma sink_trans q q' : sink q -> connect R q q' -> sink q'.
-Proof.
-move/forallP => H0 H1.
-apply/forallP => q''.
-move: (H0 q''). case_eq (f q'') => F /=;
-case_eq (connect R q' q'') => //=.
-move => H2. 
-by move: (connect_trans H1 H2) => -> //.
-Qed.
-
-Lemma final_not_sink q: f q -> ~~ sink q.
-Proof. rewrite/sink => H0. rewrite negb_forall. apply/existsP.
-exists q. rewrite negb_imply. apply/andP => //=. split.
-  by apply/connect0. 
-by apply/negPn.
-Qed.
-
-Lemma sink_not_final q: sink q -> ~~ f q.
-Proof. rewrite/sink. move/forallP => H0. 
-move: (H0 q). move: (connect0 R q) => ->.
-move/implyP => H1. exact: H1.
-Qed.
-
-
-Lemma sink_dead_end w q : sink q -> ~~ accept' q w.
-move: q. elim: w => [|a w IHw]. 
-  move => q H. apply/sink_not_final. by exact: H.
-move => q H /=. pose q' := (d q a). rewrite/accept'. simpl. fold q'.
-apply/IHw. apply/(sink_trans q) => //. apply/d_connect.
-Qed.
 
 End Acceptance.
-Implicit Arguments accept [R'].
 
 
 End DFA.
 
+(* Non-deterministic automata. These exist only
+   implicitly as non-functional transitions. *)
 Section NFA.
-Variable Q: finType.
-Variable s0: Q.
-Variable f: pred Q.
-Variable d: Q -> S -> pred Q.
-Definition Q_ndet := [ finType of {ffun Q -> bool_eqType} ].
-Definition f' (q': Q_ndet) := existsb q:Q, q' q && f q.
-Let s0' : Q_ndet := finfun (fun q:Q => q==s0).
 
-Definition d_det (q': Q_ndet) (a: S) : Q_ndet :=
-finfun (
- fun (q: Q) => existsb p: Q, q' p && d p a q
-).
+(* Usual stuff. *)
+Variable state: finType.
+Variable s0: state.
+Variable fin: pred state.
 
-Definition to_dfa : dfa Q_ndet s0' f' (dfa_rel Q_ndet d_det). constructor. Defined.
+(* Non-functional transitions. *)
+Variable step_rel: state -> char -> pred state.
+
+(* Type of states after powerset construction. *)
+Definition state_ndet := [ finType of {ffun state -> bool_eqType} ].
+
+(* Finality predicate after powerset construction. *)
+Definition fin_det := [ fun q': state_ndet => existsb q:state, q' q && fin q ].
+Definition s0_det : state_ndet := [ ffun q:state => q==s0 ].
+
+(* Functional step after powerset construction. *)
+Definition step_det := [ fun (x': state_ndet) (a: char) => 
+[ ffun x => existsb y: state, x' y && step_rel y a x ] ].
+
+(* Conversion from a non-functional transitions to a DFA. *)
+Definition to_dfa := dfaI state_ndet s0_det fin_det step_det.
+
 End NFA.
-
-
 
 End FA.
 
+Hint Unfold A_step.
+Hint Unfold A_s0.
+Hint Unfold A_fin.
 
+(* Operations on up to two automata with the same alphabet *)
 Section Operators.
-(* Operations on two automata with the same alphabet *)
-Variable Alph: finType.
-Variable Q1 Q2: finType.
-Variable s01: Q1.
-Variable s02: Q2.
-Variable f1: pred Q1.
-Variable f2: pred Q2.
+Variable char: finType.
+Variable state1 state2: finType.
+Variable s01: state1.
+Variable s02: state2.
+Variable fin1: pred state1.
+Variable fin2: pred state2.
+Variable step1: state1 -> char -> state1.
+Variable step2: state2 -> char -> state2.
 
-Variable R1': rel Q1.
-Variable R2': rel Q2.
-Variable A1: dfa Alph Q1 s01 f1 R1'.
-Variable A2: dfa Alph Q2 s02 f2 R2'.
-
-Let R1 := AutR A1.
-(*Definition d1: Q1 -> Alph -> Q1. elim: A1 => //. Defined.*)
-Definition d1 := d A1.
-Let R2 := AutR A2.
-(*Definition d2: Q2 -> Alph -> Q2. elim: A2 => //. Defined.*)
-Definition d2 := d A2.
+Variable A1: dfa char state1 s01 fin1 step1.
+Variable A2: dfa char state2 s02 fin2 step2.
 
 
-Definition q_leq {X} (q1' q2': Q_ndet X) := forall q, q1' q -> q2' q.
+(* Complement automaton *)
 
-Notation "q1' ===> q2'" := (q_leq q1' q2') (at level 70).
+(* The only change needed is to negate the finality predicate. *)
+Definition fin_not := [ fun q1 => ~~ fin1 q1 ].
+(* We construct the resulting automaton. *)
+Definition Aut_not := dfaI char state1 s01 fin_not step1.
 
-Lemma q_leq_trans {X} (q1' q2' q3': Q_ndet X) : q1' ===> q2' -> q2' ===> q3' -> q1' ===> q3'.
-Proof. rewrite/q_leq. move => H0 H1 q. by move/H0/H1. Qed.
-
-
-Definition f_not q1 := ~~ f1 q1.
-Definition Aut_not : dfa Alph Q1 s01 f_not (dfa_rel Alph Q1 d1). constructor. Defined.
-
+(* We proof that the complement automaton accepts exactly
+   the words not accepted by the original automaton. *)
 Lemma Aut_not_correct w q: accept' A1 q w = ~~ accept' Aut_not q w.
-Proof. elim: w q => [| a w IHw] q //=.
-  rewrite/f_not. by apply/idP/negPn.
+Proof.
+  by apply/idP/negPn.
 Qed.
 
-Definition f_star q1 := f1 q1 || (q1 == s01).
-Definition Q_star := Q_ndet Q1.
-Definition d_star q1 a q2 : bool := (q2 == d1 q1 a) || (f1 q1 && (q2 == d1 s01 a)).
-Definition Aut_star := to_dfa Alph Q1 s01 f_star d_star.
 
-Lemma Aut_star_correct' : accept Aut_star [::].
-Proof. rewrite/accept/accept'/f'/f_star => /=. apply/existsP. exists s01.
-by rewrite ffunE eq_refl andTb orbT. Qed.
+(* Star automaton. *)
 
-Lemma q_star_leq_d_trans (q1' q2' : Q_star) a : 
-q1' ===> q2' -> d_det Alph d_star q1' a ===> d_det Alph d_star q2' a.
-Proof. move => H0 q. rewrite/d_det. rewrite 2!ffunE. 
-move/existsP => [] p /andP [] /H0 H1 H2. apply/existsP. exists p. 
-by rewrite H1 H2. Qed.
+(* We change the finality predicate s.t. only the starthing
+   state will be accepting. *)
+Definition fin_star' := [ pred x | x == s01 ].
+(* The type of states in the star automaton. *)
+Definition state_star := state_ndet state1.
+(* We construct a non-functional relation which is 
+   the new transitions of the star automaton.
+   Whenever we enter a former final state, we
+   also enter the starting state, thereby ensuring
+   acceptance. *)
+Definition step_rel_star : state1 -> char -> pred state1 := (fun x1 a => [ pred x2 | (x2 == step1 x1 a) || (fin1 (step1 x1 a) && (x2 == s01)) ] ).
+(* We construct the star automaton. *)
+Definition Aut_star := to_dfa char state1 s01 fin_star' step_rel_star.
+Definition step_star := step_det char step_rel_star.
+Definition s0_star := s0_det state1 s01.
+Definition fin_star := fin_det state1 fin_star'.
 
-Lemma q_star_leq_eq w1 (q1' q2' : Q_star) : q1' ===> q2' -> accept' Aut_star q1' w1 -> accept' Aut_star q2' w1.
-Proof. elim: w1 q1' q2' => [|a w IHw] q1' q2'.
-  move => /=. rewrite/f'/f_star => H0 /existsP [] p /andP [] H1 /orP [] H2.
-    apply/existsP. exists p. apply/andP. split.
-      by apply: H0.
-    apply/orP. left. by exact: H2.
-  apply/existsP. exists p. apply/andP. split.
-    by apply: H0.
-  apply/orP. right. by exact: H2.
-move => H0 /=. apply: IHw.
-move: H0. exact: q_star_leq_d_trans.
+(* We proof that membership in state powerset is
+   preserved by step and step_star. *)
+Lemma step_step_star x (X: state_star) a : X x -> (step_star X a) (step1 x a).
+move => H0 /=. rewrite /step_rel_star ffunE. apply/existsP. exists x.
+rewrite H0 andTb. rewrite /SimplPred => /=. by rewrite eq_refl orTb.
 Qed.
 
-Lemma Aut_star_correct w1 w2 q1 :
-  accept' A1 q1 w1 && accept Aut_star w2 -> accept' Aut_star [ffun q => q==q1] (w1++w2).
-Proof. elim: w1 w2 q1 => [| a w1 IHw1 ] w2 q1 /andP [].
-  move => H0. apply: q_star_leq_eq.
-Admitted.
+(* Starting state correctness. *)
+Lemma Aut_star_s0 : s0_star s01. by rewrite /s0_star /s0_det ffunE eq_refl. Qed.
+
+(* step_star_rel invariant. *)
+Lemma Aut_star_step_rel (X: state_star) a: fin_star (step_star X a) -> (step_star X a) s01.
+Proof. simpl. move/existsP => [] x. by rewrite andbC => /andP [] /eqP ->. Qed.
+  
+(* We proof that the empty word is contained in the
+   language of the star automaton. *)
+Lemma Aut_star_correct0 : accept Aut_star [::].
+Proof. rewrite/accept/accept'/fin_star => /=. apply/existsP. exists s01.
+by rewrite /s0_det ffunE eq_refl. Qed.
+
+(* We proof that all non-empty words accepted by the
+   original automaton are also accepted by the star
+   automaton.
+   Translating x to [pred x' | x'==x] gives us an
+   induction hypothesis which is too weak to prove
+   the statement. Therefore, we allow the star automaton
+   to start from any set of states containing x.
+   *)
+Lemma Aut_star_correctS (X: state_star) a w x :
+  X x -> accept' A1 x (a::w) -> accept' Aut_star X (a::w).
+Proof. elim: w a X x => [| b w IHw ] a X x H0.
+  move => /= H1. apply/existsP. exists s01. rewrite ffunE eq_refl andbT.
+  apply/existsP. exists x. rewrite H0 andTb /step_rel_star /=.
+  by rewrite H1 eq_refl orbT.
+rewrite accept'S. apply: IHw. rewrite ffunE. apply/existsP. exists x.
+by rewrite H0 andTb /step_rel_star /= eq_refl.
+Qed.
+
+(* We proof that (step_star s0_star a) is a subset
+   of all (step_star X a) s.t. fin_star X. *)
+Lemma Aut_star_s0_sub X a :
+  fin_star X -> subpred (step_star s0_star a) (step_star X a).
+Proof. rewrite /fin_star/fin_det/fin_star' /s0_star/s0_det => /=. move/existsP => [] x /andP [] H0 /orP []; [ move => H1 y | move/eqP => <- y ]; rewrite ffunE;
+move/existsP => [] z; rewrite 2!ffunE /step_rel_star;
+move/andP => [] /eqP -> /= H2.
+      apply/existsP. exists s01. rewrite H2 andbT /=.
+      
+      right. by rewrite H1 andTb eq_refl.
+    move/andP => [] H2 /eqP ->. apply/existsP. exists x. rewrite H0 andTb. apply/orP.
+    right. by rewrite H1 andTb eq_refl.
+  move/eqP => ->. apply/ existsP. exists x. rewrite H0 andTb. apply/orP.
+  left. by rewrite eq_refl.
+move/andP => [] H1 /eqP ->. apply/existsP. exists x. rewrite H0 andTb.
+apply/orP. right. by rewrite H1 eq_refl.
+Qed.
+
+(* We proof that the subset relation is transitive
+   under step_star. *)
+Lemma Aut_star_subpred_trans (X Y: state_star) a : subpred X Y -> subpred (step_star X a) (step_star Y a).
+simpl. move => H0 x. rewrite 2!ffunE. move/existsP => [] y /andP [] /H0 H1 H2.
+apply/existsP. exists y. by rewrite H1 H2.
+Qed.
+
+(* We proof that powerset states accept
+   all words of all subsets *)
+Lemma Aut_star_subpred (X Y: state_star) w:
+ subpred X Y ->
+   (accept' Aut_star X) w -> (accept' Aut_star Y) w.
+Proof. elim: w X Y => [|a w IHw] X Y.
+  move => H0 /existsP [] x /andP [] /= H1 H2.
+  apply/existsP. exists x. rewrite H2 andbT.
+  apply: H0. by [].
+rewrite 2!accept'S. move => H0. apply: IHw. move: H0. by exact: Aut_star_subpred_trans.
+Qed.
+
+ 
+(* We proof that final states accept all words
+   accepted by the inital state. *) 
+Lemma Aut_star_correct' w (X: state_star) : fin_star X -> accept Aut_star w -> accept' Aut_star X w.
+Proof. elim: w X => [| a w IHw ] X. 
+  rewrite/fin_star/fin_det/ffunE. move => H0 _. simpl. rewrite /fin_star' in H0.
+  by move: H0 => /=. 
+move/(@Aut_star_s0_sub X a).
+apply: Aut_star_subpred.
+Qed.
+
+Lemma Aut_star_correct'' a w: accept Aut_star (a::w) -> exists w1, exists w2, w = w1 ++ w2 /\ accept A1 (a::w1) /\ accept Aut_star w2.
+Proof. rewrite {1}/accept {1}/accept' => /existsP [] x /andP [] H0 H1. simpl in H0.
+elim: w H0 => [|b w IHw].
+  move => H0. rewrite ffunE in H0. move/existsP: H0 => [] y /andP [] H0 H2.
+  exists [::]. exists [::]. split. by [].
+  split. simpl. rewrite/step_rel_star in H2. rewrite /s0_det ffunE in H0.
+  move/eqP: H0 H2 => H0 /=.
+  move/orP => []. move => H2. move: H1. move/eqP: H2 => ->. move: H0 => ->.
+  rewrite /fin_star' => /orP [] //.  
+  
+  rewrite Aut_star_correct0. 
+  
+
+  rewrite {1}/accept/accept' {1}[[fun _ => _] _]/=.
+elim: w => [|b w IHw].
+  simpl.
+
+  
+  
 
 
-Definition Q_prod := prod_finType Q1 Q2.
+Definition state_prod := prod_finType state1 state2.
 
-Definition d_or (q: Q_prod) a := let (q1, q2) := q in (d1 q1 a, d2 q2 a).
-Definition Aut_or : dfa Alph Q_prod (s01, s02) 
-(fun q => let (q1,q2) := q in f1 q1 || f2 q2)
-(dfa_rel Alph (Q_prod) d_or).
+Definition d_or (q: state_prod) a := let (q1, q2) := q in (step1 q1 a, step2 q2 a).
+Definition Aut_or : dfa char state_prod (s01, s02) 
+(fun q => let (q1,q2) := q in fin1 q1 || fin2 q2)
+(dfa_rel char (state_prod) d_or).
 constructor. Defined.
 
 Lemma Aut_or_correct' w q1 q2 : accept' A1 q1 w || accept' A2 q2 w = accept' Aut_or (q1, q2) w.
@@ -207,10 +296,10 @@ Lemma Aut_or_correct w: accept A1 w || accept A2 w = accept Aut_or w.
 Proof. exact: Aut_or_correct'. Qed.
 
 
-Definition d_and (q: Q_prod) a := let (q1, q2) := q in (d1 q1 a, d2 q2 a).
-Definition Aut_and : dfa Alph Q_prod (s01, s02) 
-(fun q => let (q1,q2) := q in f1 q1 && f2 q2)
-(dfa_rel Alph (Q_prod) d_or).
+Definition d_and (q: state_prod) a := let (q1, q2) := q in (step1 q1 a, step2 q2 a).
+Definition Aut_and : dfa char state_prod (s01, s02) 
+(fun q => let (q1,q2) := q in fin1 q1 && fin2 q2)
+(dfa_rel char (state_prod) d_or).
 constructor. Defined.
 
 Lemma Aut_and_correct' w q1 q2 : accept' A1 q1 w && accept' A2 q2 w = accept' Aut_and (q1, q2) w.
@@ -223,42 +312,42 @@ Qed.
 Lemma Aut_and_correct w: accept A1 w && accept A2 w = accept Aut_and w.
 Proof. exact: Aut_and_correct'. Qed.
 
-Definition Q_sum := sum_finType Q1 Q2.
-Definition Q_sum_option := option_finType Q_sum.
+Definition state_sum := sum_finType state1 state2.
+Definition state_sum_option := option_finType state_sum.
 
-Definition Q1_conc (q1: Q1) : Q_sum. constructor. exact q1. Defined.
-Definition Q2_conc (q2: Q2) : Q_sum. apply/inr. exact q2. Defined.
-Definition Q_conc := Q_ndet Q_sum.
-Definition s0_conc : Q_sum. constructor. exact: s01. Defined.
+Definition state1_conc (q1: state1) : state_sum. constructor. exact q1. Defined.
+Definition state2_conc (q2: state2) : state_sum. apply/inr. exact q2. Defined.
+Definition state_conc := state_ndet state_sum.
+Definition s0_conc : state_sum. constructor. exact: s01. Defined.
 
-Definition d_conc (q: Q_sum) a (q': Q_sum) := 
+Definition d_conc (q: state_sum) a (q': state_sum) := 
 match q with
 | inl q1 => 
   match q' with
-  | inl q1' => d1 q1 a == q1'
-  | inr q2' => f1 q1 && (d2 s02 a == q2')
+  | inl q1' => step1 q1 a == q1'
+  | inr q2' => fin1 q1 && (step2 s02 a == q2')
   end
 | inr q2 =>
   match q' with
-  | inr q2' => d2 q2 a == q2'
+  | inr q2' => step2 q2 a == q2'
   | _ => false
   end
 end.
 
-Definition f_conc (q: Q_sum) :=
+Definition f_conc (q: state_sum) :=
 match q with
-| inl q1 => f1 q1 && f2 s02
-| inr q2 => f2 q2
+| inl q1 => fin1 q1 && fin2 s02
+| inr q2 => fin2 q2
 end.
-Definition Aut_conc := to_dfa Alph Q_sum (s0_conc) f_conc d_conc. 
+Definition Aut_conc := to_dfa char state_sum (s0_conc) f_conc d_conc. 
 
-Lemma q_conc_leq_d_trans (q1' q2' : Q_conc) a : 
-q1' ===> q2' -> d_det Alph d_conc q1' a ===> d_det Alph d_conc q2' a.
-Proof. move => H0 q. rewrite/d_det. rewrite 2!ffunE. 
+Lemma q_conc_leq_d_trans (q1' q2' : state_conc) a : 
+q1' ===> q2' -> step_det char d_conc q1' a ===> step_det char d_conc q2' a.
+Proof. move => H0 q. rewrite/step_det. rewrite 2!ffunE. 
 move/existsP => [] p /andP [] /H0 H1 H2. apply/existsP. exists p. 
 by rewrite H1 H2. Qed.
 
-Lemma Aut_conc_expand1 (q1' q2': Q_conc) w:
+Lemma Aut_conc_expanstep1 (q1' q2': state_conc) w:
 q1' ===> q2' ->
 accept' Aut_conc q1' w ->
 accept' Aut_conc q2' w.
@@ -271,20 +360,20 @@ Qed.
 
 Lemma Aut_conc_correct1' q1 w1: 
 accept' A1 q1 w1 && accept A2 [::] 
--> accept' Aut_conc (finfun (fun q=> q == Q1_conc q1)) w1.
+-> accept' Aut_conc (finfun (fun q=> q == state1_conc q1)) w1.
 Proof.
 elim: w1 q1 => [|a w1 IHw1] q1.
   rewrite /f' /f_conc /accept /accept' /=.
-  move/andP => [] H0 H1. apply/existsP. exists (Q1_conc q1). 
+  move/andP => [] H0 H1. apply/existsP. exists (state1_conc q1). 
   rewrite ffunE. apply/andP. split.
     by apply/eqP.
   by rewrite H0 H1.
 move => /=. move/andP => [].
 move => H0 H1. move: (IHw1 (d A1 q1 a)). 
 rewrite H0 H1 => /=. move => H2. move: (H2 is_true_true).
-apply Aut_conc_expand1. 
+apply Aut_conc_expanstep1. 
 move => q. rewrite 2!ffunE. move/eqP => ->. apply/existsP. 
-exists (Q1_conc q1). rewrite ffunE. apply/andP. split.
+exists (state1_conc q1). rewrite ffunE. apply/andP. split.
   by apply/eq_refl.
 rewrite/d_conc => /=. by apply/eq_refl.
 Qed.
@@ -292,51 +381,51 @@ Qed.
 
 Lemma Aut_conc_correct2' q2 w2: 
 accept' A2 q2 w2
--> accept' Aut_conc (finfun (fun q=> q == Q2_conc q2)) w2.
+-> accept' Aut_conc (finfun (fun q=> q == state2_conc q2)) w2.
 Proof. elim: w2 q2 => [|a w2 IHw2] q2 /=.
-  move => H0. rewrite/f'/f_conc. apply/existsP. exists (Q2_conc q2). apply/andP. split.
+  move => H0. rewrite/f'/f_conc. apply/existsP. exists (state2_conc q2). apply/andP. split.
     by rewrite ffunE.
   by exact: H0.
-move/IHw2. apply: Aut_conc_expand1 => q. rewrite 2!ffunE. move/eqP => ->.
-apply/existsP. exists (Q2_conc q2). apply/andP. split.
+move/IHw2. apply: Aut_conc_expanstep1 => q. rewrite 2!ffunE. move/eqP => ->.
+apply/existsP. exists (state2_conc q2). apply/andP. split.
   by rewrite ffunE. 
 by rewrite/d_conc => /=.
 Qed.
 
 Lemma Aut_conc_end1 q1 a:
-f1 q1 ->
-d_det Alph d_conc [ffun q => q == Q2_conc s02] a ===> d_det Alph d_conc [ffun q => q == Q1_conc q1] a.
+fin1 q1 ->
+step_det char d_conc [ffun q => q == state2_conc s02] a ===> step_det char d_conc [ffun q => q == state1_conc q1] a.
 Proof.
-rewrite /d_det /d_conc => /=. move => H0 [q|q];
+rewrite /step_det /d_conc => /=. move => H0 [q|q];
 rewrite ffunE => /existsP [] q'; rewrite ffunE => /andP [] /eqP -> /=.
   by [].
-rewrite eq_sym ffunE => /eqP ->. apply/existsP. exists (Q1_conc q1).
+rewrite eq_sym ffunE => /eqP ->. apply/existsP. exists (state1_conc q1).
 rewrite ffunE eq_refl andTb. by rewrite H0 eq_refl.
 Qed.
 
 
 Lemma Aut_conc_correct3' q1 w2:
-f1 q1 ->
-accept' Aut_conc [ffun q => q == Q2_conc s02] w2 ->
-accept' Aut_conc [ffun q => q == Q1_conc q1] w2.
+fin1 q1 ->
+accept' Aut_conc [ffun q => q == state2_conc s02] w2 ->
+accept' Aut_conc [ffun q => q == state1_conc q1] w2.
 Proof. elim: w2 q1 => [|a w2 IHw2] q1 H0 /=.
   rewrite/f'/f_conc. move/existsP => [] q /andP []. rewrite ffunE => /eqP -> /= H1.
-  apply/existsP. exists (Q1_conc q1). by rewrite ffunE eq_refl andTb H0 H1.
+  apply/existsP. exists (state1_conc q1). by rewrite ffunE eq_refl andTb H0 H1.
 apply: Aut_conc_expand1. apply: Aut_conc_end1. by exact: H0.
 Qed.
 
 Lemma Aut_conc_correct1 q1 w1 w2: (accept' A1 q1 w1 && accept A2 w2) ->
-  accept' Aut_conc [ffun q => q == Q1_conc q1] (w1 ++ w2).
+  accept' Aut_conc [ffun q => q == state1_conc q1] (w1 ++ w2).
 Proof. elim: w1 w2 q1 => [|a w1 IHw1] w2 q1.
   rewrite/accept => /andP [] /= H0. rewrite/s0_conc. move/(Aut_conc_correct2').
-  rewrite/Q2_conc. apply: Aut_conc_correct3'. by exact: H0.
+  rewrite/state2_conc. apply: Aut_conc_correct3'. by exact: H0.
 simpl. move/IHw1. apply: Aut_conc_expand1 => q.
-rewrite /d_det /d_conc ffunE => /eqP -> /=. rewrite ffunE. apply/existsP.
-exists (Q1_conc q1). by rewrite ffunE eq_refl andTb eq_refl.
+rewrite /step_det /d_conc ffunE => /eqP -> /=. rewrite ffunE. apply/existsP.
+exists (state1_conc q1). by rewrite ffunE eq_refl andTb eq_refl.
 Qed.
 
 Lemma Aut_conc_correct2 w: 
-accept' Aut_conc [ffun q => q == Q1_conc s01] w -> 
+accept' Aut_conc [ffun q => q == state1_conc s01] w -> 
 exists w1, exists w2, w = w1 ++ w2 /\ accept A1 w1 && accept A2 w2.
 Proof. move: w.
 apply: last_ind => [| w a IHw ].
@@ -344,7 +433,7 @@ apply: last_ind => [| w a IHw ].
   exists [::]. exists [::]. rewrite/accept => /=. by rewrite H0 H1.
 case_eq (accept A1 (rcons w a)); case_eq (accept A2 [::]); move => H0 H1.
       exists (rcons w a). exists [::]. by rewrite cats0 H0 H1.
-    case_eq (accept' Aut_conc [ffun q => q == Q1_conc s01] w).
+    case_eq (accept' Aut_conc [ffun q => q == state1_conc s01] w).
       move/IHw => [] w1 [] w2 [] -> /andP [] H2 H3. rewrite rcons_cat.
       case_eq (accept A2 (rcons w2 a)) => H4.
         exists w1. exists (rcons w2 a). split.
@@ -399,8 +488,8 @@ Goal forall w q, accept' A q w -> ~~(false \in w).
 Proof. move => w. elim: w => [ | a w IHw ] //=. rewrite in_cons negb_or.
 move => q H.
 apply/andP. case: q H; case a; split; move: H => //=; try by exact: IHw.
-  move: sink_false => S; by move: (sink_dead_end A w false S) => /negbTE => -> //.
-move: sink_false => S; by move: (sink_dead_end A w false S) => /negbTE => -> //.
+  move: sink_false => char; by move: (sink_dead_end A w false char) => /negbTE => -> //.
+move: sink_false => char; by move: (sink_dead_end A w false char) => /negbTE => -> //.
 Qed.
 
 
